theories/examples.v
@@ -1,12 +1,12 @@
-From ltl Require Import ltl.
+From ltl Require Import ltl ltl_now.
+
+Import tProp.
 
 Section examples.
   Context {S L : Type}.
   Context {Rel : S → L → S → Prop}.
 
   Notation tProp := (tProp S L Rel).
-
-  Import tProp.
 
   Lemma propositional_primer (P Q R : tProp) : ⊢ (P → Q) → (Q → R) → P → R.
   Proof. iIntros "HPQ HQR HP". iDestruct ("HPQ" with "HP") as "HQ". iApply "HQR". done. Qed.
@@ -191,70 +191,6 @@ Section examples.
 
 End examples.
 
-Notation "↓s Φ" := (↓ (λ osl, (match osl with
-                              | Some (s,l) => Φ (Some s)
-                              | None => Φ None
-                              end):Prop))%I (at level 20, right associativity) : bi_scope. 
-
-Notation "↓l Φ" := (↓ (λ osl, (match osl with
-                              | Some (s,Some l) => Φ (Some l)
-                              | Some (s,None) => Φ None
-                              | None => Φ None
-                              end):Prop))%I (at level 20, right associativity) : bi_scope. 
-
-
-(* TODO! *)
-Import tProp.
-
-Inductive empty : SProp := .
-
-Class LTL (S L : Type) (Rel : S → L → S → Prop) :=
-  mkFoo
-  {
-    Rel_dec :: ∀ s l s', Decision (Rel s l s');
-  }.
-
-Definition reducible {S L} `{LTL S L} (s : S) :=
-  ∃ (l:L) (s':S), Rel s l s'.
-
-Lemma trace_steps {S L} `{HRel: LTL S L Rel} s :
-  reducible s →
-  (↓s (λ os, os = Some s)) ⊢
-  ∃ (l:L) (s':S), ⌜Rel s l s'⌝ ∧
-    ((↓l (λ ol, ol = Some l)) ∧ ○ (↓s (λ os, os = Some s'))) : tProp S L Rel.
-Proof.
-  intros (l&s'&Hsteps).
-  constructor.
-  intros [[tr|] tr_wf]; last first.
-  { unseal. rewrite ltl_now_unseal.
-    intros Hnow. inversion Hnow. simplify_eq. }
-  unseal. rewrite ltl_now_unseal.
-  intros Hnow. inversion Hnow; simplify_eq.
-  { exfalso. apply empty_ind. inversion tr_wf. subst. specialize (H0 l s'). done. }
-  clear Hsteps.
-  assert (∃ c', head_trace (Some tr0) = Some c' ∧ Rel s l0 c') as Hwf.
-  { destruct tr0.
-    { exists s0. split; [done|].
-      destruct (decide (Rel s l0 s0)); [done|].
-      exfalso. apply empty_ind. inversion tr_wf. simplify_eq.
-      simpl in *. simplify_eq. done. }
-    exists s0. split; [done|].
-    destruct (decide (Rel s l0 s0)); [done|].
-    exfalso. apply empty_ind. inversion tr_wf. simplify_eq.
-    simpl in *. simplify_eq. done. }
-  destruct Hwf as (s''&Hhead&Hrel).
-  destruct tr0; simpl in *; simplify_eq.
-  - eexists l0, s''. econstructor; [done|].
-    econstructor.
-    + econstructor. done. 
-    + rewrite ltl_next_unseal. econstructor. econstructor. done. 
-  - eexists l0, s''. econstructor; [done|].
-    econstructor.
-    + econstructor. done. 
-    + rewrite ltl_next_unseal. econstructor. econstructor. done. 
-      Unshelve. all: by inversion tr_wf.
-Qed.
-
 Section simple_ex.
   Definition state := nat.
   Definition label := unit.
@@ -271,10 +207,7 @@ Section simple_ex.
     - constructor 2. intros H. inversion H. subst. done.
   Qed.
 
-  (* TODO: Why is this needed for [unseal]? *)
-  Import tProp.
-
-  Lemma step i : ↓s (λ os, os = Some i) ⊢ ○ (↓s (λ os, os = Some (i+1))) : tProp.
+  Lemma step i : ↓s i ⊢ ○ ↓s (i+1) : tProp.
   Proof.
     iIntros "H".
     assert (∃ l s', steps i l s') as Hsteps.
@@ -285,7 +218,7 @@ Section simple_ex.
     iFrame. 
   Qed.
 
-  Lemma my_property (n:nat) : ↓s (λ os, os = Some 0) ⊢ (◊ ↓s (λ os, os = Some n)):tProp.
+  Lemma my_property (n:nat) : ↓s 0 ⊢ ◊ ↓s n : tProp.
   Proof.   
     assert (∃ i j, i = 0 ∧ n-j = i ∧ n >= j) as (i&j&<-&H1&H2).
     { eexists _, n. split; [done|]. lia. } 
@@ -309,6 +242,8 @@ Section advanced_ex.
   | my_step_succ i b : steps' (i,b) b (i+1,negb b)
   | my_step_fail i b : steps' (i,b) (negb b) (i,b).
 
+  Notation tProp := (tProp state' label' steps').
+
   Instance advanced_foo : LTL state' label' steps'.
   Proof. 
     constructor. intros.
@@ -323,15 +258,10 @@ Section advanced_ex.
   Qed.
 
   Axiom fair :
-    ∀ (b:bool), ⊢ (◊ (↓l (λ ol, ol = Some b))):tProp state' label' steps'.
-
-  (* TODO: Why is this needed for [unseal]? *)
-  Import tProp.
+    ∀ (b:bool), ⊢ ◊ ↓l b : tProp.
 
   Lemma step_b b i :
-    (↓s (λ os, os = Some (i,b))) ⊢
-    ((↓l (λ ol, ol = Some b)) ∧ ○ (↓s (λ os, os = Some (i+1,negb b)))) ∨
-      ((↓l (λ ol, ol = Some (negb b)) ∧ ○ (↓s (λ os, os = Some (i,b))))):tProp state' label' steps'.
+    ↓s (i,b) ⊢ ↓l b ∧ ○ ↓s (i+1,negb b) ∨ ↓l (negb b) ∧ ○ (↓s (i,b)) : tProp.
   Proof.
     iIntros "H".
     assert (∃ l s', steps' (i,b) l s') as Hsteps.
@@ -343,13 +273,8 @@ Section advanced_ex.
     - iRight. iFrame.
   Qed.
 
-  (* TODO: Find a better way of handling this *)
-  Lemma ltl_dup {S L Rel} (P : tProp S L Rel) : P ⊢ P ∧ P.
-  Proof. iIntros "H". iFrame. Qed.
-
   Lemma my_property'' i b :
-    ↓s (λ os, os = Some (i,b)) ⊢
-    ↓s (λ os, os = Some (i,b)) ∪ ↓s (λ os, os = Some (i+1,negb b)) : tProp state' label' steps'.
+    ↓s (i,b) ⊢ ↓s (i,b) ∪ ↓s (i+1,negb b) : tProp.
   Proof.
     iDestruct (fair b) as "-#Hfair".
     iApply (ltl_eventually_ind with "[] Hfair").
@@ -359,7 +284,7 @@ Section advanced_ex.
       iDestruct (step_b with "Hs") as "[Hs|Hs]"; last first.
       { iDestruct "Hs" as "[Hs Hs'']".
         iDestruct (ltl_now_false with "Hl Hs") as "[]".
-        destruct b; intros [[? []]|] HP HQ; by naive_solver. }
+        destruct b; intros [] [] HP HQ; by naive_solver. }
       iDestruct "Hs" as "[_ Hs'']".
       iApply ltl_until_intro_next. iFrame.
       iModIntro. iApply ltl_until_intro_now. done. }
@@ -373,7 +298,7 @@ Section advanced_ex.
   Qed.
 
   Lemma my_property' n b :
-    ↓s (λ os, os = Some (0,b)) ⊢ ∃ b, (◊ ↓s (λ os, os = Some (n,b))):tProp state' label' steps'.
+    ↓s (0,b) ⊢ ∃ b, ◊ ↓s (n,b) : tProp.
   Proof.
     assert (∃ i j, i = 0 ∧ n-j = i ∧ n >= j) as (i&j&<-&H1&H2).
     { eexists _, n. split; [done|]. lia. }
